Prove FS.v append_ok

src/FS.v
@@ -549,6 +549,62 @@ Proof.
     step.
 Qed.
 
+Definition append T fsxp inum off len (data:bytes len) mscs rx : prog T :=
+  mscs <- LOG.begin (FSXPLog fsxp) mscs;
+  let^ (mscs, ok) <- DIRTREE.append fsxp inum off data mscs;
+  If (bool_dec ok true) {
+    let^ (mscs, ok) <- LOG.commit (FSXPLog fsxp) mscs;
+    rx ^(mscs, ok)
+  } else {
+    mscs <- LOG.abort (FSXPLog fsxp) mscs;
+    rx ^(mscs, false)
+  }.
+
+Theorem append_ok: forall fsxp inum off len (newbytes:bytes len) mscs,
+   {< m pathname Fm Ftop tree Fi f bytes,
+   PRE LOG.rep (FSXPLog fsxp) (sb_rep fsxp) (NoTransaction m) mscs *
+       [[ (Fm * DIRTREE.rep fsxp Ftop tree)%pred (list2mem m) ]] *
+       [[ DIRTREE.find_subtree pathname tree = Some (DIRTREE.TreeFile inum f) ]] *
+       [[ FASTBYTEFILE.rep bytes f ]] *
+       [[ Fi (list2nmem bytes) ]] *
+       [[ goodSize addrlen (off + len) ]] *
+       (* makes this an append *)
+       [[ FASTBYTEFILE.filelen f <= off ]]
+   POST RET: ^(mscs, ok)
+       [[ ok = false ]] * LOG.rep (FSXPLog fsxp) (sb_rep fsxp) (NoTransaction m) mscs \/
+       [[ ok = true ]] *
+       exists m' tree' f' bytes' zeros,
+       LOG.rep (FSXPLog fsxp) (sb_rep fsxp) (NoTransaction m') mscs *
+       [[ (Fm * DIRTREE.rep fsxp Ftop tree')%pred (list2mem m') ]] *
+       [[ tree' = DIRTREE.update_subtree pathname (DIRTREE.TreeFile inum f') tree ]] *
+       [[ FASTBYTEFILE.rep bytes' f' ]] *
+       [[ let newdata := @Rec.of_word (Rec.ArrayF FASTBYTEFILE.byte_type len) newbytes in
+           (Fi * zeros * arrayN off newdata)%pred (list2nmem bytes')]] *
+       [[ zeros = arrayN (FASTBYTEFILE.filelen f)
+            (repeat $0 (off - (FASTBYTEFILE.filelen f))) ]]
+   CRASH LOG.would_recover_either_pred (FSXPLog fsxp) (sb_rep fsxp) m (
+       exists tree' f' bytes' zeros,
+       (Fm * DIRTREE.rep fsxp Ftop tree') *
+       [[ tree' = DIRTREE.update_subtree pathname (DIRTREE.TreeFile inum f') tree ]] *
+       [[ FASTBYTEFILE.rep bytes' f' ]] *
+       [[ let newdata := @Rec.of_word (Rec.ArrayF FASTBYTEFILE.byte_type len) newbytes in
+            (Fi * zeros * arrayN off newdata)%pred (list2nmem bytes')]] *
+       [[ zeros = arrayN (FASTBYTEFILE.filelen f)
+          (repeat $0 (off - (FASTBYTEFILE.filelen f))) ]] )
+   >} append fsxp inum off newbytes mscs.
+Proof.
+  unfold append.
+  time hoare. (* 60s *)
+  all: try rewrite LOG.activetxn_would_recover_old.
+  all: try rewrite LOG.notxn_would_recover_old.
+  all: try apply LOG.would_recover_old_either_pred.
+  rewrite <- LOG.would_recover_either_pred_pimpl.
+  cancel; eauto.
+Qed.
+
+Hint Extern 1 ({{_}} progseq (append _ _ _ _ _) _) => apply append_ok : prog.
+
+
 Definition readdir T fsxp dnum mscs rx : prog T :=
   mscs <- LOG.begin (FSXPLog fsxp) mscs;
   let^ (mscs, files) <- SDIR.dslist (FSXPLog fsxp) (FSXPBlockAlloc fsxp) (FSXPInode fsxp) dnum mscs;
